NuTest.thy
@@ -3,7 +3,7 @@ theory NuTest
 begin
 
 proc add2: "(x \<tycolon> \<nat>[32]\<heavy_comma> y \<tycolon> \<nat>[32])" \<longmapsto> "(x + x + y \<tycolon> \<nat>[32])"
-  requires [used]:"x < 100" and [used]:"y < 100"
+  requires [used]: "x < 100" and [used]:"y < 100"
   \<bullet> x x y + +
   finish
 
